added instructions to encode AT

src/Term_Defs.v
@@ -54,22 +54,23 @@ Definition Split: Set := (SP * SP).
 
 Inductive Term: Set :=
 | asp: ASP -> Term
-(*| att: Plc -> Term -> Term *)
+| att: Plc -> Term -> Term
 | lseq: Term -> Term -> Term
 (*| bseq: Split -> Term -> Term -> Term
 | bpar: Split -> Term -> Term -> Term*) .
 
 Definition LocRange: Set := list Loc.
 
-Definition getTwoLocs (ls:list Loc) (b:bool): option (Loc*Loc) :=
-  match b with
-  | true => 
+Definition getTwoLocs (ls:list Loc): option (Loc*Loc) :=
+ (* match b with
+  | true =>  *)
     match ls with
     | x :: y :: ls' => ret (x,y)
     | _ => None
-    end
+    end.
+      (*
   | false => ret (0,0)
-  end.
+  end. *)
 
 (** The structure of evidence. *)
 
@@ -101,7 +102,7 @@ Definition eval_asp t p e :=
 Fixpoint eval (t:Term) (p:Plc) (e:Evidence) : Evidence :=
   match t with
   | asp a => eval_asp a p e
-  (*| att q t1 => eval t1 q e *)
+  | att q t1 => eval t1 q e
   | lseq t1 t2 => eval t2 p (eval t1 p e)
   (*| bseq s t1 t2 => ss (eval t1 p (splitEv_T (fst s) e))
                        (eval t2 p (splitEv_T (snd s) e)) 
@@ -126,9 +127,9 @@ Inductive Ev: Set :=
 | hash: nat -> Plc -> Ev
 | req: nat -> Loc -> Plc -> Plc -> Term -> Ev
 | rpy: nat -> Loc -> Plc -> Plc -> Ev 
-| split: nat -> Plc -> Ev
+(*| split: nat -> Plc -> Ev *)
 (*| splitp: nat -> (*Loc ->*) Loc -> Plc -> Ev *)
-| join:  nat -> Plc -> Ev
+(*| join:  nat -> Plc -> Ev *)
 (*| joinp: nat -> Loc -> Loc -> Plc -> Ev *).
 
 Definition eq_ev_dec:
@@ -149,9 +150,9 @@ Definition ev x : nat :=
   | hash i _ => i
   | req i _ _ _ _ => i
   | rpy i _ _ _ => i 
-  | split i _ => i
+  (*| split i _ => i *)
   (* | splitp i _ _ => i *)
-  | join i _ => i
+  (*| join i _ => i *)
   (* | joinp i _ _ _ => i *)
   end.
 
@@ -164,9 +165,9 @@ Definition pl x : Loc :=
   | hash _ p => p
   | req _ _ p _ _ => p
   | rpy _ _ p _ => p
-  | split _ p => p
+  (*| split _ p => p *)
   (*| splitp _ _ p => p *)
-  | join _ p => p
+  (*| join _ p => p *)
   (* | joinp _ _ _ p => p *)
   end.
 
@@ -200,7 +201,7 @@ Definition Range: Set := nat * nat.
 
 Inductive AnnoTerm: Set :=
 | aasp: Range -> LocRange -> ASP -> AnnoTerm
-(*| aatt: Range -> LocRange -> (Loc*Loc) -> Plc -> AnnoTerm -> AnnoTerm *)
+| aatt: Range -> LocRange -> (Loc*Loc) -> Plc -> AnnoTerm -> AnnoTerm
 | alseq: Range -> LocRange -> AnnoTerm -> AnnoTerm -> AnnoTerm
 (*| abseq: Range -> LocRange -> Split -> AnnoTerm -> AnnoTerm -> AnnoTerm
 | abpar: Range -> LocRange -> (*(Loc*Loc) ->*) (Loc*Loc) -> Split -> AnnoTerm -> AnnoTerm -> AnnoTerm*) .
@@ -208,7 +209,7 @@ Inductive AnnoTerm: Set :=
 Fixpoint esize t :=
   match t with
   | aasp _ _ _ => 1
-  (*| aatt _ _ _ _ t1 => 2 + (*remote_esize t1*) esize t1 *)
+  | aatt _ _ _ _ t1 => 2 + (*remote_esize t1*) esize t1
   | alseq _ _ t1 t2 => esize t1 + esize t2
   (*| abseq _ _ _ t1 t2 => 2 + esize t1 + esize t2
   | abpar _ _ _ _ t1 t2 => 2 + esize t1 + esize t2 *)
@@ -217,7 +218,7 @@ Fixpoint esize t :=
 Definition range x :=
   match x with
   | aasp r _ _ => r
-  (*| aatt r _ _ _ _ => r *)
+  | aatt r _ _ _ _ => r
   | alseq r _ _ _ => r
   (*| abseq r _ _ _ _ => r
   | abpar r _ _ _ _ _ => r *)
@@ -226,7 +227,7 @@ Definition range x :=
 Definition lrange x :=
   match x with
   | aasp _ lr _ => lr
-  (*| aatt _ lr _ _ _ => lr *)
+  | aatt _ lr _ _ _ => lr
   | alseq _ lr _ _ => lr
   (*| abseq _ lr _ _ _ => lr
   | abpar _ lr _ _ _ _ => lr *)
@@ -235,7 +236,7 @@ Definition lrange x :=
 Fixpoint anss (t:AnnoTerm) :=
   match t with
   | aasp _ _ _ => 0
-  (* | aatt _ _ _ _ t => 2 (* + (remote_anss t) (*(anss t) + 2*) *) *)
+  | aatt _ _ _ _ t => 2 + anss t (* + (remote_anss t) (*(anss t) + 2*) *)
   | alseq _ _ t1 t2 => anss t1 + anss t2
   (*| abseq _ _ _ t1 t2 => anss t1 + anss t2
   | abpar _ _ _ _ t1 t2 => 2 + anss t1 + anss t2 *)
@@ -245,11 +246,25 @@ Fixpoint anss (t:AnnoTerm) :=
 Fixpoint nss (t:Term) :=
   match t with
   | asp _ => 0
-  (*| att _ t => (*nss t +*) 2 *)
+  | att _ t => nss t + 2
   | lseq t1 t2 => nss t1 + nss t2
   (*| bseq _ t1 t2 => nss t1 + nss t2
   | bpar  _ t1 t2 => 2 + nss t1 + nss t2 *)
   end.
+
+Definition two_ats := (att 1 (att 2 (asp (CPY)))).
+Compute nss two_ats.
+Compute nss (lseq two_ats two_ats).
+
+Definition three_ats := (att 1 (att 2 (att 3 (asp (CPY))))).
+Compute nss three_ats.
+
+Definition three_ats' := (att 1 (lseq (asp CPY) (att 2 (att 3 (asp (CPY)))))).
+Compute nss three_ats'.
+
+Definition four_ats := (lseq (att 1 (lseq (asp CPY) three_ats))
+                             (att 2 (att 1 (asp CPY)))).
+Compute nss four_ats.
 
 Lemma nss_even: forall t n,
     nss t = n ->
@@ -262,10 +277,13 @@ Proof.
       cbn in *;
       subst;
       tauto.
-    (*
+    
   -
     cbn in *.
-    eauto. *)
+    subst.
+    
+    assert (Nat.even (nss t) = true) by eauto.
+    eapply both_args_even; eauto.
   -
     cbn in *.
     subst.
@@ -292,21 +310,19 @@ Defined.
     throughout the computation so as to ensure each event has a unique
     natural number. *) *)
 
-Fixpoint anno (t: Term) (i:nat) (ls:LocRange) (b:bool) : option (nat * (* (LocRange **) AnnoTerm)(* ) *) :=
+Fixpoint anno (t: Term) (i:nat) (ls:LocRange) (*(b:bool)*) : option (nat * (* (LocRange **) AnnoTerm)(* ) *) :=
   match t with
   | asp x => ret (S i, (aasp (i, S i) [] x))
 
-  (*| att p x =>
-    '(req_loc,rpy_loc) <- getTwoLocs ls b ;;
-    '(j,a) <- anno x (S i) [] false  ;;
+  | att p x =>
+    '(req_loc,rpy_loc) <- getTwoLocs ls ;;
+    '(j,a) <- anno x (S i) (skipn 2 ls) (* false*)  ;;
     (* TODO: does ls matter here?  Should it be []? *)
-    ret (S j, aatt (i, S j) (firstn 2 ls) (req_loc,rpy_loc) p a) 
-   *)
+    ret (S j, aatt (i, S j) ls (*(firstn 2 ls)*) (req_loc,rpy_loc) p a) 
                 
-
   | lseq x y =>
-    '(j,a) <- anno x i (firstn (nss x) ls) b  ;;
-    '(k,bt) <- anno y j (skipn (nss x) ls ) b  ;;
+    '(j,a) <- anno x i (firstn (nss x) ls) ;;
+    '(k,bt) <- anno y j (skipn (nss x) ls ) ;;
     ret (k, alseq (i, k) ls (*(lrange a ++ lrange bt)*) a bt)
 
         (*
@@ -325,7 +341,7 @@ Fixpoint anno (t: Term) (i:nat) (ls:LocRange) (b:bool) : option (nat * (* (LocRa
 *)
   end.
 
-Definition anno' t i ls := fromSome (0, aasp (0,0) [] CPY) (anno t i ls true).
+Definition anno' t i ls := fromSome (0, aasp (0,0) [] CPY) (anno t i ls).
 
 Definition annotated x ls :=
   snd (anno' x 0 ls).
@@ -333,7 +349,7 @@ Definition annotated x ls :=
 Fixpoint unanno a :=
   match a with
   | aasp _ _ a => asp a
-  (*| aatt _ _ _ p t => att p (unanno t) *)
+  | aatt _ _ _ p t => att p (unanno t)
   | alseq _ _ a1 a2 => lseq (unanno a1) (unanno a2)
                          
   (*| abseq _ _ spl a1 a2 => bseq spl (unanno a1) (unanno a2) 
@@ -360,12 +376,12 @@ Inductive well_formed_r: AnnoTerm -> Prop :=
 | wf_asp_r: forall r x ls,
     snd r = S (fst r) ->
     well_formed_r (aasp r ls x)
-(*| wf_att_r: forall r ls locs p x,
+| wf_att_r: forall r ls locs p x,
     well_formed_r x ->
     S (fst r) = fst (range x) ->
     snd r = S (snd (range x)) ->
-    Nat.pred (snd r) > fst r ->
-    well_formed_r (aatt r ls locs p x) *)
+    (*Nat.pred (snd r) > fst r -> *)
+    well_formed_r (aatt r ls locs p x)
                   
 | wf_lseq_r: forall r ls x y,
     well_formed_r x -> well_formed_r y ->
@@ -394,11 +410,12 @@ Inductive well_formed: AnnoTerm -> Prop :=
 | wf_asp: forall r x,
     snd r = S (fst r) ->
     well_formed (aasp r [] x)
-(*| wf_att: forall r ls locs p x,
-    well_formed_r x ->
+| wf_att: forall r ls locs p x,
+    (*well_formed_r x -> *)
+    well_formed x ->
     S (fst r) = fst (range x) ->
     snd r = S (snd (range x)) ->
-    Nat.pred (snd r) > fst r ->
+    (*Nat.pred (snd r) > fst r -> *)
 
     
     fst locs <> snd locs ->
@@ -417,7 +434,7 @@ Inductive well_formed: AnnoTerm -> Prop :=
      *)
     
     
-    well_formed (aatt r ls locs p x) *)
+    well_formed (aatt r ls locs p x)
                 
 | wf_lseq: forall r ls x y,
     well_formed x -> well_formed y ->
