src/Main.v
@@ -27,11 +27,11 @@ Inductive traceS: St -> list Ev -> Prop :=
 | tconf: forall t tr p e,
     trace t p tr ->
     traceS (conf t p e) tr
-(*| trem: forall st tr j loc p,
+| trem: forall st tr j loc p,
     traceS st tr ->
     traceS (rem j loc p st)
            (tr ++
-               [(rpy (pred j) loc p (pl st))]) *)
+               [(rpy (pred j) loc p (pl st))])
 | tls: forall st tr1 t tr2,
     traceS st tr1 ->
     trace t (pl st) tr2 ->
@@ -57,7 +57,7 @@ Fixpoint esizeS s:=
   match s with
   | stop _ _ => 0
   | conf t _ _ => esize t
-  (*| rem _ _ _ st => 1 + esizeS st *)
+  | rem _ _ _ st => 1 + esizeS st
   | ls st t => esizeS st + esize t
   (*| bsl _ st t _ _ => 1 + esizeS st + esize t
   | bsr _ _ st => 1 + esizeS st
@@ -168,7 +168,7 @@ Proof.
     (*
     inv H2; auto. *)
 
-    (*
+    
   -
 
     (*
@@ -201,7 +201,6 @@ Proof.
      *)
 
     eauto.
-*)
 
   -
 
@@ -317,13 +316,13 @@ Proof.
   - constructor.
     constructor.
 
-    (*
+    
     
   - constructor. apply tatt. simpl.
     solve_by_inversion.
     (*
     inv H6; auto. *)
-*)
+
 
     (*
   - constructor. apply tbseq; auto.
@@ -337,7 +336,7 @@ Proof.
     inv H6; auto. inv H7; auto. *)
 
      *)
-    (*
+    
   -
     find_copy_apply_lem_hyp step_seval.
     find_copy_apply_lem_hyp step_pl_eq.
@@ -356,10 +355,10 @@ Proof.
     eapply IHst in H7; eauto.
     (* rewrite <- G. *) rewrite <- G1.
     rewrite app_comm_cons; auto. *)
-     *)
-    (*
+     
+    
   - rewrite <- app_nil_l; auto.
-    apply trem; auto. *)
+    apply trem; auto. 
   -
     find_copy_apply_lem_hyp step_seval.
     find_copy_apply_lem_hyp step_pl_eq.
